cava/Cava/Acorn/Acorn.v
@@ -17,7 +17,6 @@
 Require Export Cava.Acorn.CavaClass.
 Require Export Cava.Signal.
 Require Export Cava.Acorn.CombinationalMonad.
-Require Export Cava.Acorn.Sequential.
 Require Export Cava.Acorn.Combinators.
 Require Export Cava.Acorn.NetlistGeneration.
 Require Export Cava.Acorn.CavaPrelude.
