cava/Cava/Extraction.v
@@ -30,7 +30,6 @@ Require Import Cava.Signal.
 Require Import Cava.VectorUtils.
 Require Import Cava.Acorn.Acorn.
 Require Import Cava.Acorn.CombinationalMonad.
-Require Import Cava.Acorn.Sequential.
 Require Import Cava.Acorn.CavaClass.
 Require Import Cava.Acorn.Combinators.
 Require Import Cava.Acorn.NetlistGeneration.
@@ -45,7 +44,6 @@ Recursive Extraction Library BitArithmetic.
 Recursive Extraction Library Cava.
 Recursive Extraction Library Acorn.
 Recursive Extraction Library CombinationalMonad.
-Recursive Extraction Library Sequential.
 Recursive Extraction Library Combinators.
 Recursive Extraction Library NetlistGeneration.
 
